proof/refine/ARM_HYP/ArchBits_R.thy
@@ -12,8 +12,6 @@ context Arch begin arch_global_naming
 
 clear_named_theorems Arch_assms (* accumulate assumptions for Bits_R locale *)
 
-crunch_ignore (add: setCurrentPD)
-
 lemma atcbContext_get_eq[Arch_assms, simp]:
   "atcbContextGet (atcbContextSet x atcb) = x"
   by (simp add: atcbContextGet_def atcbContextSet_def)
